rich_raven_lang/trnsl.v
@@ -57,6 +57,12 @@ Section MainTranslation.
       expr_step e (symb_stk_to_stk_frm stk mp) (Val (trnsl_lval lv)).
     Admitted.
 
+    Lemma trnsl_expr_interp_lexpr_compatibility2 stk e lexpr lv mp : 
+      trnsl_expr_lExpr stk e = Some (lexpr) -> 
+      expr_step e (symb_stk_to_stk_frm stk mp) (Val (trnsl_lval lv)) ->
+      interp_lexpr lexpr mp = Some lv.
+    Admitted.
+
     Definition trnsl_hoare_triple (stk_id: stack_id) (p : assertion) (msk : maskAnnot) (cmd : stmt) (q : assertion) (mp : symb_map) : iProp rrl_lang.Σ :=
         match (trnsl_stmt cmd) with 
         | Error => True
@@ -183,18 +189,45 @@ Section MainTranslation.
           rewrite HstkI. simpl. done.
     Qed.
 
-  
-    Theorem rrl_validity stk_id p msk cmd q :
-      stmt_well_defined cmd -> 
-      forall mp, ⌜RavenHoareTriple p cmd msk q⌝
-      ⊢ (trnsl_hoare_triple stk_id p msk cmd q mp).
+
+    Axiom proc_specs_valid :
+      forall proc proc_record stk_vals, 
+      proc ∈ proc_set  ->
+      proc_map !! proc = Some proc_record ->
+
+      exists (ret_val: lang.val),
+      forall precond postcond stk_id stk_frm mp stmt mask,
+
+      (forall v, v ∈ (proc_args_of proc_record) -> is_Some (stk_frm.(locals) !! v.1)) ->
+
+      Forall2 (λ var val, stk_frm.(locals) !! var = Some val) (proc_args_of proc_record).*1 stk_vals ->
+
+      
+
+      let subst_map' := list_to_map (zip (proc_args_of proc_record).*1 (map (λ val, LVal (trnsl_val val)) stk_vals)) in
+
+
+      trnsl_assertion (subst (proc_precond_of proc_record) subst_map') stk_id mp = Some precond ->
+      trnsl_assertion (subst (proc_postcond_of proc_record) (<["#ret_val" := LVal (trnsl_val (ret_val))]> subst_map')) stk_id mp = Some postcond ->
+      
+      ((trnsl_stmt (proc_body_of proc_record) = Some' stmt) \/ (trnsl_stmt (proc_body_of proc_record) = None' /\ stmt = lang.SkipS) ) ->
+      (∃ stk_frm'',
+      ({{{ stack_own[stk_id, stk_frm] ∗ precond }}} (to_rtstmt stk_id stmt) @ mask {{{ RET lang.LitUnit; stack_own[stk_id, stk_frm''] ∗ ⌜ (locals stk_frm'' !! "#ret_val") = Some ret_val ⌝ ∗ postcond }}})).
+
+    
+
+    Theorem rrl_validity ρ σ stk_id p msk cmd q :
+      stmt_well_defined ρ cmd -> 
+      forall mp, (env_typ_well_defined σ mp) ->
+       ⌜RavenHoareTriple ρ σ p cmd msk q⌝
+      ⊢  (trnsl_hoare_triple stk_id p msk cmd q mp).
     Proof.
-      iIntros (Hwelldef mp) "%H". 
+      iIntros (Hwelldef mp Henv) "%H". 
       iInduction H as 
       [ | 
-      | stk mask v fld e old_val new_val lv Hatm HLexpr1 
+      | ρ σ stk mask v fld e old_val new_val lv Hatm HLexpr1 
       | | | | 
-      | stk mask invr args stmt inv_record p q lexprs Hargs Hinv_mask Hinv_record subst Hbody IHHbody
+      | ρ σ stk mask invr args stmt inv_record p q lexprs Hargs Hinv_mask Hinv_record Hstk_tp subst Hbody IHHbody
       | | | | | | | | ] "IH".
       3: { 
         (* FIELD WRITE *)
@@ -282,7 +315,7 @@ Section MainTranslation.
           (* Unset Printing Notations. *)
           (* iPoseProof IHHbody as "Htriple". *)
           
-          iPoseProof ("IH" with  "[%] Hcomb") as "IH2". { done. }
+          iPoseProof ("IH" with  "[%] [%] Hcomb") as "IH2"; try done.
           iFrame.
           assert ((inv_set_to_namespace (mask ∖ {[invr]})) = inv_set_to_namespace mask ∖ ↑inv_namespace_map invr) as HInvs. { admit. }
           rewrite HInvs.
@@ -322,7 +355,7 @@ Section MainTranslation.
           rewrite H1; destruct H1.
 
           inversion Hwelldef as [ | | | | | | | | | | | | | inv args' stmt' HInvSet HargsWellDef HBodywelldef | ]; subst stmt' args'.
-          iApply ("IH" with "[%] Hcomb"). { done. }
+          iApply ("IH" with "[%] [%] Hcomb"); try done.
           iNext.
           iIntros "[Hstk [Hu Hu1]]".
           iModIntro.
@@ -378,10 +411,10 @@ Section MainTranslation.
                   destruct (stk !! i) as [x|] eqn:HstkI;  simpl; auto.
                   + assert (x ≠ lv). { specialize (H0 i). rewrite HstkI in H0. intros Heq. subst x. contradiction.
                   } simpl.
-                  rewrite HstkI. simpl. f_equal. rewrite <- String.eqb_neq in H1. rewrite H1. auto.
+                  rewrite HstkI. simpl. f_equal. rewrite <- String.eqb_neq in H2. rewrite H2. auto.
 
                   + rewrite HstkI. simpl. done.
-              } rewrite H1. done.
+              } rewrite H2. done.
 
           }
           iPureIntro.
@@ -405,7 +438,7 @@ Section MainTranslation.
           destruct (trnsl_assertion p stk_id mp) eqn:Hp, (trnsl_assertion q stk_id mp) eqn:Hq, (trnsl_assertion r stk_id mp) eqn:Hr; try done. 
 
           iIntros "[Hu Hu1]".
-          iPoseProof ("IH2" with "Hu") as ">IH3". iModIntro; iFrame.
+          iPoseProof ("IH2" with "[%] Hu") as ">IH3"; try done. iModIntro; iFrame.
 
         }
 
@@ -413,7 +446,7 @@ Section MainTranslation.
         
         iIntros (Φ).
         iModIntro. iIntros "[Hu Hu1] HΦ".
-        iApply ("IH2" with "Hu").
+        iApply ("IH2" with "[%] Hu"); try done.
         iNext. iIntros "Hu0". iApply "HΦ". iFrame.
         }
       }
@@ -444,7 +477,7 @@ Section MainTranslation.
           simpl in H1.
           assert (l = {| loc_car := loc_car l |}).
           { destruct l. simpl. done.  }
-          rewrite H2. done. 
+          rewrite H3. done. 
         }
 
         {
@@ -463,7 +496,7 @@ Section MainTranslation.
             iFrame; iPureIntro.
             pose proof (fresh_var_trnsl_expr_invariant stk lvar_x e _ mp val H0 H).
             unfold LExpr_holds.
-            simpl. rewrite <- H1. apply HLe_h.
+            simpl. rewrite <- H2. apply HLe_h.
           
             + iPureIntro. unfold LExpr_holds. simpl. rewrite String.eqb_refl. rewrite val_beq_refl. done.
         }
@@ -488,12 +521,12 @@ Section MainTranslation.
           
           + simpl. iFrame. rewrite fresh_mp_rewrite_symb_stk_to_stk_frm_compat; try done.
           unfold symb_stk_to_stk_frm. simpl. 
-          assert (lang.LitLoc l = lang.LitLoc {| loc_car := loc_car l |}) as H0.
+          assert (lang.LitLoc l = lang.LitLoc {| loc_car := loc_car l |}) as H1.
           {  destruct l. simpl. done. }
-          rewrite <- H0. iFrame.
+          rewrite <- H1. iFrame.
 
           + simpl. destruct a as [fld val].
-          assert (stmt_well_defined (Alloc x fld_vals)) as Hwell_def'. { admit. }
+          assert (stmt_well_defined ρ (Alloc x fld_vals)) as Hwell_def'. { admit. }
           destruct (trnsl_assertion (field_list_to_assertion (LVar lvar_x) fld_vals) stk_id mp' ) eqn:Htrfl.
           
             * simpl. rewrite Htrfl.
@@ -502,16 +535,17 @@ Section MainTranslation.
             iDestruct "Hhp" as "[Hhpl Hhpfvs]".
             iPoseProof ("IH2" with "Hstk Hhpfvs") as "[IH3 IH3']". 
             iFrame. iExists l. 
-            assert (trnsl_lval (trnsl_val val) = val) as H0. { admit. } 
-            rewrite H0. iFrame.
+            assert (trnsl_lval (trnsl_val val) = val) as H1. { admit. } 
+            rewrite H1. iFrame.
             iPureIntro. 
             unfold LExpr_holds.
             simpl.
             subst mp'. simpl. rewrite String.eqb_refl. rewrite val_beq_refl. done.
 
-            * simpl. rewrite Htrfl. iPoseProof ("IH" with "[%]") as "IH2"; try done. iClear "IH".
+            * simpl. rewrite Htrfl. iPoseProof ("IH" with "[%]") as "IH2"; try done.
+             (* iClear "IH".
             iDestruct "Hhp" as "[Hhpl Hhp2]". 
-            iApply ("IH2" with "Hstk Hhp2").  
+            iApply ("IH2" with "Hstk Hhp2").   *)
       }
 
 
@@ -528,7 +562,7 @@ Section MainTranslation.
         (* FOLD PRED *)
         unfold trnsl_hoare_triple.
         simpl.
-        pose proof (trnsl_pred_validity pred lexprs stk_id mp) as HPredTrnsl. rewrite H0 in HPredTrnsl. unfold subst_map in HPredTrnsl. rewrite HPredTrnsl.
+        pose proof (trnsl_pred_validity pred lexprs stk_id mp) as HPredTrnsl. rewrite H1 in HPredTrnsl. unfold subst_map in HPredTrnsl. rewrite HPredTrnsl.
         iIntros. iModIntro.  iFrame.
       }
 
@@ -544,19 +578,22 @@ Section MainTranslation.
         destruct (trnsl_assertion a2 stk_id mp) eqn:Ha2.
         - destruct (trnsl_stmt c1) eqn:Hc1, (trnsl_stmt c2) eqn:Hc2; try done.
           + destruct (trnsl_assertion a1 stk_id mp) eqn:Ha1, (trnsl_assertion a3 stk_id mp) eqn: Ha3; try done. iIntros "Hu0".
-          iPoseProof ("IH'" with "Hu0") as ">IHH".
-           iApply "IH1'". iFrame.
+          iPoseProof ("IH'" with "[%] Hu0") as ">IHH"; try done.
+           iApply "IH1'"; try done.
 
           + destruct (trnsl_assertion a1 stk_id mp) eqn:Ha1, (trnsl_assertion a3 stk_id mp) eqn: Ha3; try done. 
             iIntros (Φ). iModIntro. iIntros "Hu0 HΦ".
-            iPoseProof ("IH'" with "Hu0") as ">IHH".
-            iApply ("IH1'" with "IHH"); iFrame.
+            iPoseProof ("IH'" with "[%] Hu0") as ">IHH"; try done.
+            iApply ("IH1'" with "[%] IHH"); try done.
 
           + destruct (trnsl_assertion a1 stk_id mp) eqn:Ha1, (trnsl_assertion a3 stk_id mp) eqn: Ha3; try done. admit.
 
           + destruct (trnsl_assertion a1 stk_id mp) eqn:Ha1, (trnsl_assertion a3 stk_id mp) eqn: Ha3; try done.
           simpl.
-          iApply wp_seq; try done.
+          iApply wp_seq.
+            { iApply "IH'"; try done. }
+            { iApply "IH1'"; try done. }
+
 
         - admit.
            (* Case: trnsl_assertion a2 = None; *)
@@ -600,7 +637,7 @@ Section MainTranslation.
         
         { assert (trnsl_lval (LitLoc l) = (lang.LitLoc l)).
         - simpl. destruct l. simpl. done.
-        - rewrite -> H3 in *. done. }
+        - rewrite -> H4 in *. done. }
 
         { iFrame. }
 
@@ -651,8 +688,8 @@ Section MainTranslation.
 
         iApply (wp_cas_fail v e1 fld e2 e3 stk_id (symb_stk_to_stk_frm stk mp) l (trnsl_lval old_val2) (trnsl_lval old_val) _ with "[Hstk Hl]"); try done.
         
-        - assert (trnsl_lval (LitLoc l) = (lang.LitLoc l)) as H2. { simpl. destruct l. simpl. done. }
-        { rewrite -> H2 in *. done. }
+        - assert (trnsl_lval (LitLoc l) = (lang.LitLoc l)) as H3. { simpl. destruct l. simpl. done. }
+        { rewrite -> H3 in *. done. }
 
         - unfold LExpr_holds in Hneq.
           simpl in Hneq. injection Hneq as Hneq.
@@ -707,14 +744,14 @@ Section MainTranslation.
         iPoseProof ("IH" with "[%]") as "IH2"; try done.
         iIntros "HP'".
         iApply HQ_ent_Q'.
-        iApply "IH2".
+        iApply "IH2"; try done.
         iApply HP_ent_P'.
         iFrame.
 
         -
         iPoseProof ("IH" with "[%]") as "IH2"; try done.
         iIntros (Φ). iModIntro. iIntros "HP' HΦ".
-        iApply ("IH2" with "[HP']").
+        iApply ("IH2" with "[%] [HP']"); try done.
           + iApply HP_ent_P'. iFrame.
           + iNext. iIntros "HQ". iApply "HΦ". iApply HQ_ent_Q'. iFrame.
       }
@@ -727,20 +764,369 @@ Section MainTranslation.
         iClear "IH IH1".
         unfold trnsl_hoare_triple. simpl.
 
+        pose proof (lexpr_expr_typ_compat _ _ _ _ _ _ H1 H H0) as Hlexpr_type_inf.
+          pose proof (lexpr_typcheck_well_defined _ _ _ _ Henv Hlexpr_type_inf) as Hinterp_lexpr.
+          destruct Hinterp_lexpr as [val0 Hinterp_lexpr].
+          pose proof (interp_lexpr_typ_compat _ _ _ _ _ Henv Hlexpr_type_inf Hinterp_lexpr) as Hle_typ.
+          unfold typeOf in Hle_typ. destruct (trnsl_lval val0) eqn:Hle_val; try done.
+          unfold trnsl_lval in Hle_val. destruct (val0) eqn: Hle_val'; try done.
+
         destruct (trnsl_stmt s1) eqn:Hs1, (trnsl_stmt s2) eqn:Hs2; try done;
 
         destruct (trnsl_assertion p stk_id mp) eqn:HP, (trnsl_assertion q stk_id mp) eqn:HQ; try done.
 
-        - iFrame.
-        admit.
+        - destruct b0.
 
-        - admit.
-
-        - admit.
-
-        - admit.
-
+          + iIntros "[Hstk Hu]".
+          iApply "IH'"; try done. iFrame. iPureIntro.
+          unfold LExpr_holds. rewrite Hinterp_lexpr. done.
+          
+          + iIntros "[Hstk Hu]".
+          iApply "IH1'"; try done. iFrame. iPureIntro.
+          unfold LExpr_holds. simpl. rewrite Hinterp_lexpr. done.
         
+
+        - iIntros (Φ). iModIntro. iIntros "[Hstk Hu] HΦ".
+          destruct b0.
+          + iApply (wp_if_t e (RTSkipS stk_id) (to_rtstmt stk_id s) stk_id (symb_stk_to_stk_frm stk1 mp) u (stack_own[ stk_id, symb_stk_to_stk_frm stk2 mp] ∗ u0) (lang.LitUnit) (inv_set_to_namespace mask) with "[IH'] [IH' Hstk Hu ] [HΦ]"); try iFrame.
+            *  apply (trnsl_expr_interp_lexpr_compatibility _ e lexpr (LitBool true) mp); try done.
+
+            * iIntros (Φ'). iModIntro. iIntros "[Hstk Hu] HΦ'".
+            iPoseProof ("IH'" with "[%] [Hstk Hu]" ) as "HQ"; try done; try iFrame.
+            { iPureIntro. unfold LExpr_holds. rewrite Hinterp_lexpr. done.  }
+            iMod "HQ". iApply (wp_skip (stack_own[ stk_id, symb_stk_to_stk_frm stk2 mp] ∗ u0) with "[HQ]"); iFrame.
+
+            
+          
+          + iApply (wp_if_f e (RTSkipS stk_id) (to_rtstmt stk_id s) stk_id (symb_stk_to_stk_frm stk1 mp) u (stack_own[ stk_id, symb_stk_to_stk_frm stk2 mp] ∗ u0) (lang.LitUnit) (inv_set_to_namespace mask) with "[IH'] [IH' Hstk Hu ] [HΦ]"); try iFrame.
+            * apply (trnsl_expr_interp_lexpr_compatibility _ e lexpr (LitBool false) mp); try done.
+
+            * iIntros (Φ'). iModIntro. iIntros "[Hstk Hu] HΦ'".
+            iPoseProof ("IH1'" with "[%] [Hstk Hu]" ) as "HQ"; try done; try iFrame.
+            { iPureIntro. unfold LExpr_holds. simpl. rewrite Hinterp_lexpr. done.  }
+            iApply "HQ"; iFrame.
+            
+
+        - iIntros (Φ). iModIntro. iIntros "[Hstk Hu] HΦ".
+          destruct b0.
+          + iApply (wp_if_t e (to_rtstmt stk_id s) (RTSkipS stk_id) stk_id (symb_stk_to_stk_frm stk1 mp) u (stack_own[ stk_id, symb_stk_to_stk_frm stk2 mp] ∗ u0) (lang.LitUnit) (inv_set_to_namespace mask) with "[IH'] [IH' Hstk Hu ] [HΦ]"); try iFrame.
+            *  apply (trnsl_expr_interp_lexpr_compatibility _ e lexpr (LitBool true) mp); try done.
+
+            * iIntros (Φ'). iModIntro. iIntros "[Hstk Hu] HΦ'".
+            iPoseProof ("IH'" with "[%] [Hstk Hu]" ) as "HQ"; try done; try iFrame.
+            { iPureIntro. unfold LExpr_holds. rewrite Hinterp_lexpr. done.  }
+            iApply "HQ"; iFrame.
+            
+
+            
+          
+          + iApply (wp_if_f e (to_rtstmt stk_id s) (RTSkipS stk_id) stk_id (symb_stk_to_stk_frm stk1 mp) u (stack_own[ stk_id, symb_stk_to_stk_frm stk2 mp] ∗ u0) (lang.LitUnit) (inv_set_to_namespace mask) with "[IH'] [IH' Hstk Hu ] [HΦ]"); try iFrame.
+            * apply (trnsl_expr_interp_lexpr_compatibility _ e lexpr (LitBool false) mp); try done.
+
+            * iIntros (Φ'). iModIntro. iIntros "[Hstk Hu] HΦ'".
+            iPoseProof ("IH1'" with "[%] [Hstk Hu]" ) as "HQ"; try done; try iFrame.
+            { iPureIntro. unfold LExpr_holds. simpl. rewrite Hinterp_lexpr. done.  }
+            iMod "HQ". iApply (wp_skip (stack_own[ stk_id, symb_stk_to_stk_frm stk2 mp] ∗ u0) with "[HQ]"); iFrame.
+
+        - iIntros (Φ). iModIntro. iIntros "[Hstk Hu] HΦ".
+          destruct b0.
+          + iApply (wp_if_t e (to_rtstmt stk_id s) (to_rtstmt stk_id s0) stk_id (symb_stk_to_stk_frm stk1 mp) u (stack_own[ stk_id, symb_stk_to_stk_frm stk2 mp] ∗ u0) (lang.LitUnit) (inv_set_to_namespace mask) with "[IH'] [IH' Hstk Hu ] [HΦ]"); try iFrame.
+            *  apply (trnsl_expr_interp_lexpr_compatibility _ e lexpr (LitBool true) mp); try done.
+
+            * iIntros (Φ'). iModIntro. iIntros "[Hstk Hu] HΦ'".
+            iPoseProof ("IH'" with "[%] [Hstk Hu]" ) as "HQ"; try done; try iFrame.
+            { iPureIntro. unfold LExpr_holds. rewrite Hinterp_lexpr. done.  }
+            iApply "HQ"; iFrame.
+            
+
+            
+          
+          + iApply (wp_if_f e (to_rtstmt stk_id s) (to_rtstmt stk_id s0) stk_id (symb_stk_to_stk_frm stk1 mp) u (stack_own[ stk_id, symb_stk_to_stk_frm stk2 mp] ∗ u0) (lang.LitUnit) (inv_set_to_namespace mask) with "[IH'] [IH' Hstk Hu ] [HΦ]"); try iFrame.
+            * apply (trnsl_expr_interp_lexpr_compatibility _ e lexpr (LitBool false) mp); try done.
+
+            * iIntros (Φ'). iModIntro. iIntros "[Hstk Hu] HΦ'".
+            iPoseProof ("IH1'" with "[%] [Hstk Hu]" ) as "HQ"; try done; try iFrame.
+            { iPureIntro. unfold LExpr_holds. simpl. rewrite Hinterp_lexpr. done.  }
+            iApply "HQ"; iFrame.
+
+      }
+      
+      1 : {
+        (* CALL *)
+        unfold trnsl_hoare_triple. simpl (trnsl_stmt (Call x proc_name args)). case_match; try discriminate.
+        pose proof H0 as H0'.
+        apply proc_args_unique in H0'.
+        pose proof H0 as Hspec_StackFree.
+        apply proc_spec_stack_free in Hspec_StackFree.
+
+        destruct (trnsl_assertion (LAnd (LStack stk) (LAnd (LProc proc_name proc_record) (subst (proc_precond_of proc_record) subst_map))) stk_id mp) eqn:HPreCond; try done.
+
+        destruct (trnsl_assertion
+          (LExists lvar_x
+          (LAnd (LStack (<[x:=lvar_x]> stk))
+          (subst (proc_postcond_of proc_record) (<["#ret_var":=LVar lvar_x]> subst_map)))) stk_id mp
+        ) eqn:HPostCond; try done.
+
+        inversion Hwelldef; subst ρ0 v proc args0.
+
+        assert (exists arg_vals, Forall2 (fun e v => expr_step e (symb_stk_to_stk_frm stk mp) (Val v)) args arg_vals) as Harg_vals.
+
+        { 
+          (* Prove existence of arg_vals *)
+          clear Hwelldef H1 H4 H11.
+          clear subst_map HPreCond HPostCond.
+          revert lexprs H2 H12. 
+          induction args as [| a args IH]; intros lexprs H2 H12.
+          - simpl in H2. destruct lexprs; [ | discriminate ]. exists nil. constructor.
+          - simpl in H2. destruct lexprs as [| l lexprs']; [ discriminate | ].
+            (* heads must match and tails must match *)
+            simpl in H2. injection H2 as Hhd Htl.
+            inversion H12 as [| a' args' Hwd H12']. clear H12; subst.
+            (* interp_lexpr either yields a value or None *)
+            destruct (interp_lexpr l mp) as [v | ] eqn:He.
+            + (* Some v: build the head step and recurse for the tail *)
+              specialize (IH lexprs' Htl H12') as [arg_vals' Hforall'].
+              exists ((trnsl_lval v) :: arg_vals').
+              apply Forall2_cons. split.
+              * apply trnsl_expr_interp_lexpr_compatibility with (lexpr:=l); try assumption.
+              * exact Hforall'.
+            + (* None: contradict well-definedness using expr_interp_well_defined *)
+              eapply (expr_interp_well_defined stk a mp l) in Hhd; [ | exact He ].
+              congruence.
+        }
+
+        destruct Harg_vals as [arg_vals Harg_vals].
+
+        assert (Forall2 (λ expr val, interp_lexpr expr mp = Some (trnsl_val val)) lexprs arg_vals) as Hlexprs_arg_vals.
+          {
+            clear   Hwelldef H1  H4 H11 H12 subst_map HPreCond HPostCond.
+            revert args arg_vals H2 Harg_vals.
+            induction lexprs as [| le lexprs IH]; intros args arg_vals H2 Harg_vals.
+            - destruct args; [| discriminate]. inversion Harg_vals. constructor.
+
+            - destruct args; [discriminate |]. simpl in H2. injection H2 as Hhd Htl.
+              inversion Harg_vals as [ | x0 y l l' HhdExprStep HtlExprStep ]; subst.
+              specialize (IH args l' Htl HtlExprStep).
+              apply Forall2_cons. split.
+              + apply (trnsl_expr_interp_lexpr_compatibility2 stk e); try simpl; try done. rewrite trnsl_lval_trnsl_val_inverse. done.
+
+              + done.
+          }
+
+        simpl in *.
+        destruct proc_record as [proc_args proc_locals proc_pre proc_post proc_body] eqn:Hproc_record.
+        destruct (trnsl_stmt (proc_body)) eqn:Hproc_body, (trnsl_assertion (subst proc_pre subst_map) stk_id mp) eqn:Hproc_pre; try rewrite Hproc_pre in HPreCond;  try discriminate; simpl in HPreCond.
+        
+        {   
+          (* proc_body = Skip *)
+        inversion H4; subst s. inversion HPreCond; subst u; clear HPreCond.
+        inversion HPostCond as [ HPostCond']; clear HPostCond.
+        iIntros (Φ). iModIntro.
+        
+        iIntros "[Hstk [Hproc_tbl Hu1]] HΦ".
+
+        (* pose proof (proc_specs_valid proc_name (Proc proc_args proc_locals proc_pre proc_post proc_body) u1 u0 stk_id' mp lang.SkipS (inv_set_to_namespace mask) stk_frm' arg_vals) as [ret_val Hproc]. *)
+
+        (* destruct HPostCond' as [ret_val HPostCond]. *)
+
+        pose proof (proc_specs_valid proc_name (Proc proc_args proc_locals proc_pre proc_post proc_body) arg_vals ) as [ret_val Hproc]; try done.
+
+        set (subst_map' := @list_to_map var LExpr (gmap var LExpr) _ _ (zip (proc_args).*1 (map (λ val, LVal (trnsl_val val)) arg_vals))).
+
+          destruct (trnsl_assertion (subst proc_pre subst_map') stk_id mp) as [ proc_frame_pre |] eqn: Hproc_frame_pre.
+          
+          2 : {  
+            (* trnsl_assertion (subst proc_pre subst_map') stk_id' mp CANNOT BE None *)
+            admit.
+          }
+
+          destruct (trnsl_assertion (subst proc_post (<["#ret_val":=LVal (trnsl_val ret_val)]> subst_map')) stk_id mp) as [ proc_frame_post |] eqn: Hproc_frame_post.
+
+          2 : {
+            (* trnsl_assertion (subst proc_pre subst_map') stk_id' mp CANNOT BE None *)
+            admit. 
+          }
+
+        iApply (wp_call _ _ _ _ _ _ _ (lang.Proc proc_name proc_args proc_locals _) _ u1 proc_frame_post with "[] [Hstk Hproc_tbl Hu1]"); try iFrame; try done.
+
+          { 
+            (* Showing procedure contract holds *)
+            iIntros (stk_id' stk_frm') "%HlocalsDef". simpl in *.
+
+            specialize (Hproc proc_frame_pre proc_frame_post stk_id' stk_frm' mp lang.SkipS(inv_set_to_namespace mask)).
+
+            assert ((∀ v : var * typ, v ∈ proc_args_of (Proc proc_args proc_locals proc_pre proc_post proc_body) → is_Some (locals stk_frm' !! v.1))) as HIsSome.
+
+            { 
+              intros v Hin. apply elem_of_list_lookup_1 in Hin as [i Hi].
+              assert (proc_args.*1 !! i = Some v.1) as Hi'.
+              { rewrite list_lookup_fmap. rewrite Hi. done.   } 
+              simpl in HlocalsDef.
+              eapply (Forall2_lookup_l _ proc_args.*1 arg_vals i v.1 HlocalsDef) in Hi' as [val [Hval Hlookup]]. by eexists.
+            }
+
+          pose proof (Hproc HIsSome) as Hproc. simpl in Hproc.
+
+          simpl in HlocalsDef. pose proof (Hproc HlocalsDef) as Hproc.
+
+          rewrite (stack_free_assertion_trnsl (subst proc_pre subst_map') stk_id stk_id' mp) in Hproc_frame_pre. 2 : { apply stack_free_assertion_subst. destruct Hspec_StackFree; done. }
+
+          rewrite (stack_free_assertion_trnsl (subst proc_post (<["#ret_val":=LVal (trnsl_val ret_val)]> subst_map')) stk_id stk_id' mp) in Hproc_frame_post. 2 : { apply stack_free_assertion_subst. destruct Hspec_StackFree; done. }
+
+          pose proof (Hproc Hproc_frame_pre Hproc_frame_post) as Hproc.
+
+          assert (trnsl_stmt proc_body = Some' lang.SkipS
+            ∨ trnsl_stmt proc_body = None' ∧ lang.SkipS = lang.SkipS) as Hproc_body'. { right. split; try done. }
+          
+          pose proof (Hproc Hproc_body') as Hproc.
+
+          destruct Hproc as [stk_frm'' Hproc].
+
+          iExists stk_frm''.
+          
+          iIntros (Φ'). iModIntro.
+          iIntros "[Hstk Hu1] HΦ".
+
+          iApply (Hproc with "[Hstk Hu1]").
+
+          { 
+            rewrite (stack_free_assertion_trnsl (subst proc_pre subst_map') stk_id' stk_id mp) in Hproc_frame_pre. 2 : { apply stack_free_assertion_subst. destruct Hspec_StackFree as [Hpre_stack_free _]. done. }
+
+
+            iFrame.
+            pose proof (trnsl_assertion_w_lexpr_subst proc_pre lexprs proc_args.*1 arg_vals stk_id mp u1 proc_frame_pre Hlexprs_arg_vals Hproc_pre Hproc_frame_pre) as Himpl.
+            iApply Himpl. iFrame.
+          }
+
+          
+          iNext. iExact "HΦ".
+
+
+          }
+
+          {
+            iNext. iIntros "[Hstk Hq]".
+            iApply "HΦ". iExists (trnsl_val ret_val).
+          
+            destruct (trnsl_assertion (subst proc_post (<["#ret_var":=LVar lvar_x]> subst_map)) stk_id
+            (λ x0 : lvar, if (x0 =? lvar_x)%string then trnsl_val ret_val else mp x0)) 
+            eqn:Hpost; try done.
+            
+            iSplitR "Hq". 
+            { rewrite fresh_mp_rewrite_symb_stk_to_stk_frm_compat; try done. rewrite trnsl_lval_trnsl_val_inverse. iFrame. } 
+            
+            { pose proof (trnsl_assertion_w_lexpr_subst_r proc_post lexprs proc_args.*1 arg_vals lvar_x ret_val stk stk_id mp u proc_frame_post H Hlexprs_arg_vals Hpost Hproc_frame_post) as Himpl. iApply Himpl. iFrame. }
+            
+            
+          }
+
+        }
+
+
+        {   
+          (* proc_body != Skip *)
+        inversion H4; subst s. inversion HPreCond; subst u; clear HPreCond.
+        inversion HPostCond as [ HPostCond']; clear HPostCond.
+        iIntros (Φ). iModIntro.
+        
+        iIntros "[Hstk [Hproc_tbl Hu1]] HΦ".
+
+        (* pose proof (proc_specs_valid proc_name (Proc proc_args proc_locals proc_pre proc_post proc_body) u1 u0 stk_id' mp lang.SkipS (inv_set_to_namespace mask) stk_frm' arg_vals) as [ret_val Hproc]. *)
+
+        (* destruct HPostCond' as [ret_val HPostCond]. *)
+
+        pose proof (proc_specs_valid proc_name (Proc proc_args proc_locals proc_pre proc_post proc_body) arg_vals ) as [ret_val Hproc]; try done.
+
+        set (subst_map' := @list_to_map var LExpr (gmap var LExpr) _ _ (zip (proc_args).*1 (map (λ val, LVal (trnsl_val val)) arg_vals))).
+
+          destruct (trnsl_assertion (subst proc_pre subst_map') stk_id mp) as [ proc_frame_pre |] eqn: Hproc_frame_pre.
+          
+          2 : {  
+            (* trnsl_assertion (subst proc_pre subst_map') stk_id' mp CANNOT BE None *)
+            admit.
+          }
+
+          destruct (trnsl_assertion (subst proc_post (<["#ret_val":=LVal (trnsl_val ret_val)]> subst_map')) stk_id mp) as [ proc_frame_post |] eqn: Hproc_frame_post.
+
+          2 : {
+            (* trnsl_assertion (subst proc_pre subst_map') stk_id' mp CANNOT BE None *)
+            admit. 
+          }
+
+        iApply (wp_call _ _ _ _ _ _ _ (lang.Proc proc_name proc_args proc_locals _) _ u1 proc_frame_post with "[] [Hstk Hproc_tbl Hu1]"); try iFrame; try done.
+
+          { 
+            (* Showing procedure contract holds *)
+            iIntros (stk_id' stk_frm') "%HlocalsDef". simpl in *.
+
+            specialize (Hproc proc_frame_pre proc_frame_post stk_id' stk_frm' mp s0 (inv_set_to_namespace mask)).
+
+            assert ((∀ v : var * typ, v ∈ proc_args_of (Proc proc_args proc_locals proc_pre proc_post proc_body) → is_Some (locals stk_frm' !! v.1))) as HIsSome.
+
+            { 
+              intros v Hin. apply elem_of_list_lookup_1 in Hin as [i Hi].
+              assert (proc_args.*1 !! i = Some v.1) as Hi'.
+              { rewrite list_lookup_fmap. rewrite Hi. done.   } 
+              simpl in HlocalsDef.
+              eapply (Forall2_lookup_l _ proc_args.*1 arg_vals i v.1 HlocalsDef) in Hi' as [val [Hval Hlookup]]. by eexists.
+            }
+
+          pose proof (Hproc HIsSome) as Hproc. simpl in Hproc.
+
+          simpl in HlocalsDef. pose proof (Hproc HlocalsDef) as Hproc.
+
+          rewrite (stack_free_assertion_trnsl (subst proc_pre subst_map') stk_id stk_id' mp) in Hproc_frame_pre. 2 : { apply stack_free_assertion_subst. destruct Hspec_StackFree; done. }
+
+          rewrite (stack_free_assertion_trnsl (subst proc_post (<["#ret_val":=LVal (trnsl_val ret_val)]> subst_map')) stk_id stk_id' mp) in Hproc_frame_post. 2 : { apply stack_free_assertion_subst. destruct Hspec_StackFree; done. }
+
+          pose proof (Hproc Hproc_frame_pre Hproc_frame_post) as Hproc.
+
+          assert (trnsl_stmt proc_body = Some' s0
+            ∨ trnsl_stmt proc_body = None' ∧ s0 = lang.SkipS) as Hproc_body'. { left. try done. }
+          
+          pose proof (Hproc Hproc_body') as Hproc.
+
+          destruct Hproc as [stk_frm'' Hproc].
+
+          iExists stk_frm''.
+          
+          iIntros (Φ'). iModIntro.
+          iIntros "[Hstk Hu1] HΦ".
+
+          iApply (Hproc with "[Hstk Hu1]").
+
+          { 
+            rewrite (stack_free_assertion_trnsl (subst proc_pre subst_map') stk_id' stk_id mp) in Hproc_frame_pre. 2 : { apply stack_free_assertion_subst. destruct Hspec_StackFree as [Hpre_stack_free _]. done. }
+
+
+            iFrame.
+            pose proof (trnsl_assertion_w_lexpr_subst proc_pre lexprs proc_args.*1 arg_vals stk_id mp u1 proc_frame_pre Hlexprs_arg_vals Hproc_pre Hproc_frame_pre) as Himpl.
+            iApply Himpl. iFrame.
+          }
+
+          
+          iNext. iExact "HΦ".
+
+
+          }
+
+          {
+            iNext. iIntros "[Hstk Hq]".
+            iApply "HΦ". iExists (trnsl_val ret_val).
+          
+            destruct (trnsl_assertion (subst proc_post (<["#ret_var":=LVar lvar_x]> subst_map)) stk_id
+            (λ x0 : lvar, if (x0 =? lvar_x)%string then trnsl_val ret_val else mp x0)) 
+            eqn:Hpost; try done.
+            
+            iSplitR "Hq". 
+            { rewrite fresh_mp_rewrite_symb_stk_to_stk_frm_compat; try done. rewrite trnsl_lval_trnsl_val_inverse. iFrame. } 
+            
+            { pose proof (trnsl_assertion_w_lexpr_subst_r proc_post lexprs proc_args.*1 arg_vals lvar_x ret_val stk stk_id mp u proc_frame_post H Hlexprs_arg_vals Hpost Hproc_frame_post) as Himpl. iApply Himpl. iFrame. }
+            
+            
+          }
+
+        }
 
       }
 
